src/Axioms.v
@@ -1,0 +1,3 @@
+Require Import Coq.Logic.ClassicalFacts.
+
+Axiom prop_ext: prop_extensionality.
